WIP switcher interp

theories/examples/switcher/switcher_spec.v
@@ -2,7 +2,7 @@ From iris.algebra Require Import frac excl_auth.
 From iris.proofmode Require Import proofmode.
 From cap_machine Require Import logrel fundamental interp_weakening addr_reg_sample rules proofmode.
 From cap_machine Require Import multiple_updates region_invariants_revocation region_invariants_allocation.
-From cap_machine Require Import switcher.
+From cap_machine Require Import switcher switcher_preamble.
 
 
 
@@ -22,180 +22,6 @@ Section Switcher.
   Notation WORLD := ( prodO (prodO STS_STD STS) TFRAME) .
   Implicit Types W : WORLD.
   Implicit Types C : CmptName.
-
-  (** Property of capability sealed by the switcher's otype *)
-  Definition export_tableN (C : CmptName) : namespace := nroot .@ "export_tableN" .@ C.
-  Definition export_table_PCCN (C : CmptName) : namespace := (export_tableN C) .@ "PCC".
-  Definition export_table_CGPN (C : CmptName) : namespace := (export_tableN C) .@ "CGP".
-  Definition export_table_entryN (C : CmptName) (a : Addr) : namespace :=
-    (export_tableN C) .@ "entry" .@ a.
-
-  Program Definition execute_entry_point_register (wpcc wcgp : Word) :
-    (WORLD -n> (leibnizO CmptName) -n> (leibnizO Reg) -n> iPropO Σ) :=
-    λne (W : WORLD) (C : CmptName) (reg : leibnizO Reg),
-      (full_map reg ∧
-       ⌜ reg !! PC = Some wpcc ⌝ ∧
-       ⌜ reg !! cgp = Some wcgp ⌝ ∧
-       (∀ (wstk : Word), (⌜reg !! csp = Some wstk⌝ → interp W C wstk)) ∧
-       (∀ (wret : Word), (⌜reg !! cra = Some wret⌝ → interp W C wret)) ∧
-       (∀ (r : RegName) (v : Word), (⌜r ∈ dom_arg_rmap⌝ → ⌜reg !! r = Some v⌝ → interp W C v)) ∧
-       (∀ (r : RegName),
-          (⌜r ∉ (dom_arg_rmap ∪ {[PC; cra; cgp; csp]})⌝ →  ⌜reg !! r = Some (WInt 0)⌝)))%I.
-  Solve All Obligations with solve_proper.
-
-  Program Definition execute_entry_point (wpcc wcgp : Word) (regs : Reg) : (WORLD -n> (leibnizO CmptName) -n> iPropO Σ) :=
-    (λne (W : WORLD) (C : CmptName),
-       ( (execute_entry_point_register wpcc wcgp W C regs)
-         ∗ registers_pointsto regs
-         ∗ region W C
-         ∗ sts_full_world W C
-         ∗ tframe_frag (frm W)
-         ∗ na_own logrel_nais ⊤
-           -∗ interp_conf W C)
-    )%I.
-  Solve All Obligations with solve_proper.
-
-  Program Definition ot_switcher_prop :
-    (WORLD -n> (leibnizO CmptName) -n> (leibnizO Word) -n> iPropO Σ):=
-    λne (W : WORLD) (C : CmptName) (w : Word),
-       (∃ (g_tbl : Locality) (b_tbl e_tbl a_tbl : Addr)
-          (bpcc epcc : Addr)
-          (bcgp ecgp : Addr)
-          (nargs off : Z),
-           ⌜ w = WCap RO g_tbl b_tbl e_tbl a_tbl ⌝
-           ∗ ⌜ (b_tbl <= a_tbl < e_tbl)%a ⌝
-           ∗ ⌜ (b_tbl < (b_tbl ^+1))%a ⌝
-           ∗ ⌜ ((b_tbl ^+1) < a_tbl)%a ⌝
-           ∗ ⌜ (0 <= nargs <= 7 )%Z ⌝
-           ∗ inv (export_table_PCCN C) ( b_tbl ↦ₐ WCap RX Global bpcc epcc bpcc)
-           ∗ inv (export_table_CGPN C) ( (b_tbl ^+ 1)%a ↦ₐ WCap RW Global bcgp ecgp bcgp)
-           ∗ inv (export_table_entryN C a_tbl) ( a_tbl ↦ₐ WInt (encode_entry_point nargs off))
-           ∗ □ ( ∀ W' regs, ⌜related_sts_priv_world W W'⌝ →
-                   ▷ (execute_entry_point
-                            (WCap RX Global bpcc epcc (bpcc ^+ off)%a)
-                            (WCap RW Global bcgp ecgp bcgp)
-                            regs W' C))
-      )%I.
-  Solve All Obligations with solve_proper.
-
-  Definition ot_switcher_propC : (WORLD * CmptName * Word) -> iPropI Σ :=
-    safeC ot_switcher_prop.
-
-  Lemma persistent_cond_ot_switcher :
-    persistent_cond ot_switcher_prop.
-  Proof. intros [ [] ] ; cbn ; apply _. Qed.
-
-  Lemma mono_priv_ot_switcher (C : CmptName) (w : Word) :
-    ⊢ future_priv_mono C ot_switcher_propC w.
-  Proof.
-    iIntros (W W' Hrelated_W_W').
-    iModIntro.
-    iIntros "Hot_switcher".
-    iEval (cbn) in "Hot_switcher".
-    iEval (cbn).
-    iDestruct "Hot_switcher" as
-      (g_tbl b_tbl e_tbl a_tbl bpcc epcc bcgp ecgp nargs off ->
-       Hatbl Hbtbl Hbtbl1 Hnargs) "(Hinvpcc & Hinvcgp & Hinventry & #Hcont)".
-    iFrame "Hinvpcc Hinvcgp Hinventry".
-    iExists _,_.
-    repeat (iSplit ; first done).
-    iModIntro.
-    iIntros (W'' regs Hrelated_W'_W'').
-    iSpecialize ("Hcont" $! W'' regs).
-    iApply "Hcont".
-    iPureIntro.
-    by eapply related_sts_priv_trans_world.
-  Qed.
-
-  (** Custom invariant used by the switcher to store the frame  *)
-   Definition frame_inv (C : CmptName) (i : positive) (P : iProp Σ) :=
-     (∃ x:bool, sts_state_loc C i x ∗ if x then P else emp)%I.
-   Definition frame_rel_pub := λ (a b : bool), False.
-   Definition frame_rel_priv := λ (a b : bool), True.
-   Definition frame_W (W : WORLD) : WORLD :=
-     let ι := fresh_cus_name W in
-      <l[ ι := true , ( frame_rel_pub, (frame_rel_pub, frame_rel_priv)) ]l> W.
-
-   Lemma frame_W_related_sts_pub_world (W : WORLD) : related_sts_pub_world W (frame_W W).
-   Proof.
-     rewrite /frame_W.
-     destruct W as [ [Wstd [fs fr] ] Wfrm ] .
-     assert (fresh (dom fs ∪ dom fr) ∉ (dom fs ∪ dom fr)) as Hfresh by apply is_fresh.
-     apply related_sts_pub_world_fresh_loc; set_solver.
-   Qed.
-
-   Set Nested Proofs Allowed.
-
-  Lemma frame_W_lookup_std (W : WORLD) (a : Addr) :
-    std (frame_W W) !! a = (std W) !!a.
-  Proof.
-    rewrite /frame_W.
-    by cbn.
-  Qed.
-
-  Lemma frame_W_lookup_loc (W : WORLD) (ι : positive) :
-    ι ≠ fresh_cus_name W ->
-    loc (frame_W W) !! ι = (loc W) !! ι.
-  Proof.
-    intros Hι.
-    rewrite /frame_W /= lookup_insert_ne //.
-  Qed.
-  Lemma frame_W_lookup_rel (W : WORLD) (ι : positive) :
-    ι ≠ fresh_cus_name W ->
-    wrel (frame_W W) !! ι = (wrel W) !! ι.
-  Proof.
-    intros Hι.
-    rewrite /frame_W /= lookup_insert_ne //.
-  Qed.
-  Lemma frame_W_lookup_frm (W : WORLD) : frm (frame_W W) = (frm W).
-  Proof. by cbn. Qed.
-
-  Lemma ι0_in_Wloc_helper (W0 : WORLD) (ι0 : positive) (callee_stk_frm_addr : list Addr) :
-    ι0 ∈ (dom (loc (std_update_multiple
-                       (<l[ι0:=false]l>(revoke W0))
-                       callee_stk_frm_addr Temporary))).
-  Proof.
-    rewrite std_update_multiple_loc_sta dom_insert_L; set_solver.
-  Qed.
-
-  Lemma ι0_isnot_fresh (W0 : WORLD) (ι0 : positive) (callee_stk_frm_addr : list Addr) :
-    ι0 ≠ fresh_cus_name (std_update_multiple
-                           (<l[ι0:=false]l>(revoke W0))
-                           callee_stk_frm_addr Temporary).
-  Proof.
-    apply fresh_name_notin. left.
-    apply ι0_in_Wloc_helper.
-  Qed.
-
-
-  (** Evolution of the world in the switcher *)
-  Definition switcher_world_pre_frame (W_init : WORLD) (callee_stk_frm_addr : list Addr) :=
-    (std_update_multiple (<d[ frm W_init + 1]d>(revoke W_init)) callee_stk_frm_addr Temporary).
-
-  Definition switcher_world_upon_jmp (W_init : WORLD)
-    (a_local_args callee_stk_frm_addr : list Addr) :=
-    std_update_multiple
-      (frame_W (switcher_world_pre_frame W_init callee_stk_frm_addr))
-      a_local_args Temporary.
-
-  Lemma related_sts_priv_world_switcher_pre_frame
-    (W : WORLD) (callee_stk_frm_addr : list Addr) :
-    Forall (fun a => std W !! a = Some Revoked) callee_stk_frm_addr ->
-    related_sts_priv_world W (switcher_world_pre_frame W callee_stk_frm_addr).
-  Proof.
-    intros Ha_local_args.
-    rewrite /switcher_world_pre_frame.
-    eapply related_sts_priv_trans_world; cycle 1.
-    { apply related_sts_pub_priv_world.
-      apply related_sts_pub_update_multiple_temp.
-      eapply Forall_impl; eauto.
-      intros a Ha; cbn in *.
-      by apply revoke_lookup_Revoked.
-    }
-    eapply related_sts_priv_trans_world; cycle 1.
-    { apply sts.related_sts_priv_world_update_frm. }
-    apply revoke_related_sts_priv_world.
-  Qed.
 
   Lemma switcher_world_pre_frame_local_revoked
     (W : WORLD) (callee_stk_frm_addr : list Addr) (a : Addr) :
@@ -510,22 +336,6 @@ Section Switcher.
              apply rtc_refl.
   Qed.
 
-  Definition switcher_inv
-    (b_switcher e_switcher a_switcher_cc b_tstk e_tstk : Addr)
-    (ot_switcher : OType) : iProp Σ :=
-    ∃ (a_tstk : Addr) (d : nat) (tstk_next : list Word),
-     mtdc ↦ₛᵣ WCap RWL Local b_tstk e_tstk a_tstk
-     ∗ ⌜ SubBounds
-         b_switcher e_switcher
-         a_switcher_cc (a_switcher_cc ^+ length switcher_instrs)%a ⌝
-     ∗ ⌜ (ot_switcher < (ot_switcher ^+1) )%ot ⌝
-     ∗ codefrag a_switcher_cc switcher_instrs
-     ∗ b_switcher ↦ₐ WSealRange (true,true) Global ot_switcher (ot_switcher^+1)%ot ot_switcher
-     ∗ [[ (a_tstk ^+1)%a, e_tstk ]] ↦ₐ [[ tstk_next ]]
-     ∗ ⌜ (b_tstk <= a_tstk)%a ∧ (a_tstk <= e_tstk)%a ⌝
-     ∗ tframe_full d ∗ ⌜ (b_tstk + d)%a = Some a_tstk  ⌝
-     ∗ seal_pred ot_switcher ot_switcher_propC.
-
   Lemma switcher_ret_specification
     (Nswitcher Nframes : namespace)
     (W0 : WORLD)
@@ -578,7 +388,7 @@ Section Switcher.
     in
 
     Nswitcher ## Nframes ->
-    (a_switcher_cc + 79%nat)%a = Some a_jmp ->
+    (a_switcher_cc + 85%nat)%a = Some a_jmp ->
     (a_stk ^+ 3 < e_stk)%a ->
     (b_stk <= a_stk)%a ->
     (a_tstk ^+ 1 < e_tstk)%a ->
@@ -682,7 +492,6 @@ Section Switcher.
 
     (* ReadSR ctp mtdc *)
     iInstr "Hcode".
-    { done. }
 
     (* TODO extract as lemma about frame_W *)
     iDestruct (sts_full_state_loc with "[$] [$Hι_loc]") as "%Hι_state".
@@ -737,7 +546,6 @@ Section Switcher.
     { by transitivity (Some a_tstk); solve_addr. }
     (* WriteSR mtdc ctp *)
     iInstr "Hcode".
-    { done. }
     (* Lea csp (-1)%Z *)
     iInstr "Hcode".
     { by transitivity (Some (a_stk ^+ 3)%a); solve_addr. }
@@ -1289,22 +1097,30 @@ Section Switcher.
     (* ---- lea csp 1 ---- *)
     iInstr "Hcode".
     { transitivity (Some (a_stk ^+ 4%Z)%a); auto;solve_addr. }
-
     (* --- getp ct2 csp --- *)
     iInstr "Hcode".
-
     (* --- mov ctp (encodePerm RWL) --- *)
     iInstr "Hcode".
-
     (* --- sub ct2 ct2 ctp --- *)
     iInstr "Hcode".
     replace ((encodePerm RWL - encodePerm RWL)%Z) with 0%Z by lia.
-
     (* --- jnz 2 ct2 --- *)
     iInstr "Hcode".
-
     (* --- jmp 2 --- *)
     iInstr "Hcode".
+
+    (* --- getl ct2 csp --- *)
+    iInstr "Hcode".
+    (* --- mov ctp (encodeLoc Local) --- *)
+    iInstr "Hcode".
+    (* --- sub ct2 ct2 ctp --- *)
+    iInstr "Hcode".
+    replace ((encodeLoc Local - encodeLoc Local)%Z) with 0%Z by lia.
+    (* --- jnz 2 ct2 --- *)
+    iInstr "Hcode".
+    (* --- jmp 2 --- *)
+    iInstr "Hcode".
+
 
     (* --- readsr ct2 mtdc --- *)
     iInstr "Hcode".
@@ -1364,7 +1180,6 @@ Section Switcher.
 
     (* WriteSR mtdc ct2; *)
     iInstr "Hcode".
-    { done. (* TODO add to solve_pure *) }
 
     (* Zero out the callee's stack frame *)
     (* GetE cs0 csp; *)
