theories/examples/switcher/switcher_interp.v
@@ -2,7 +2,7 @@ From iris.algebra Require Import frac excl_auth.
 From iris.proofmode Require Import proofmode.
 From cap_machine Require Import logrel fundamental interp_weakening addr_reg_sample rules proofmode.
 From cap_machine Require Import multiple_updates region_invariants_revocation region_invariants_allocation.
-From cap_machine Require Import switcher switcher_spec.
+From cap_machine Require Export switcher switcher_preamble.
 
 Section Switcher.
   Context
@@ -45,6 +45,235 @@ Section Switcher.
     iExists _,_; iFrame "∗%".
   Qed.
 
+  Lemma writeLocalAllowed_valid_cap (W : WORLD) (C : CmptName) p g b e a':
+    isWL p = true →
+    interp W C (WCap p g b e a') -∗
+    ⌜Forall (fun a => std W !! a = Some Temporary ) (finz.seq_between b e)⌝.
+  Proof.
+    iIntros (Hwa) "Hinterp".
+    rewrite Forall_forall.
+    iIntros (a Ha).
+    apply elem_of_finz_seq_between in Ha.
+    rewrite /interp; cbn.
+    rewrite fixpoint_interp1_eq interp1_eq; cbn.
+    replace (isO p) with false.
+    2: { eapply isWL_nonO in Hwa ;done. }
+    destruct (has_sreg_access p) eqn:HnXSR; auto.
+    iDestruct "Hinterp" as "[Hinterp %Hloc]".
+    iDestruct (extract_from_region_inv with "Hinterp")
+             as (p' P' Hfl' Hpers') "(Hrel & Hzcond & Hrcond & Hwcond & HmonoR & %Hstate)";eauto.
+    iPureIntro.
+    destruct (isWL p); simplify_eq.
+    by rewrite /region_state_pwl in Hstate.
+  Qed.
+
+  Lemma wp_store_interp (E : coPset) (W : WORLD) (C : CmptName) (rsrc rdst : RegName)
+    (pc_p : Perm) (pc_g : Locality) (pc_b pc_e pc_a pc_a' : Addr)
+    (p : Perm) (g : Locality) (b e a a' : Addr)
+    (wi wsrc : Word)
+    :
+    decodeInstrW wi = Store rdst (inr rsrc) →
+    isCorrectPC (WCap pc_p pc_g pc_b pc_e pc_a) →
+    (pc_a + 1)%a = Some pc_a' →
+
+     {{{ interp W C wsrc
+           ∗ interp W C (WCap p g b e a')
+           ∗ PC ↦ᵣ WCap pc_p pc_g pc_b pc_e pc_a
+           ∗ pc_a ↦ₐ wi
+           ∗ rsrc ↦ᵣ wsrc
+           ∗ rdst ↦ᵣ WCap p g b e a
+           ∗ region W C
+           ∗ sts_full_world W C
+     }}}
+       Instr Executable @ E
+       {{{ retv, RET retv;
+           ⌜ retv = FailedV ⌝ ∨
+          ( ⌜ retv = NextIV ⌝
+           ∗ PC ↦ᵣ WCap pc_p pc_g pc_b pc_e pc_a'
+           ∗ pc_a ↦ₐ wi
+           ∗ rsrc ↦ᵣ wsrc
+           ∗ rdst ↦ᵣ WCap p g b e a
+           ∗ region W C
+           ∗ sts_full_world W C
+           ∗ ⌜ canStore p wsrc = true ⌝
+           ∗ ⌜(b <= a < e)%a ⌝
+          )
+       }}}.
+  Proof.
+    iIntros (Hdecode_wi Hcorrect_pc Hpca' φ)
+      "(#Hinterp_src & #Hinterp_dst & HPC & Hi & Hsrc & Hdst & Hregion & Hworld)".
+    iIntros "Hφ".
+
+    destruct (decide (canStore p wsrc = true))%a as [Hstore_src|Hstore_src]; cycle 1.
+    {
+      iApply (wp_store_fail_reg_perm with "[HPC Hi Hdst Hsrc]")
+      ; try iFrame
+      ; try solve_pure.
+      { by destruct ( canStore p wsrc ); auto. }
+      iNext; iIntros "_".
+      iApply "Hφ"; by iLeft.
+    }
+    pose proof ( canStore_writeAllowed p wsrc Hstore_src ) as Hp_stk_wa.
+    destruct (decide (b <= a))%a as [Hba|Hba]; cycle 1.
+    {
+      iApply (wp_store_fail_reg with "[HPC Hi Hdst Hsrc]")
+      ; try iFrame
+      ; try solve_pure.
+      { rewrite /withinBounds; solve_addr. }
+      iNext; iIntros "_".
+      iApply "Hφ"; by iLeft.
+    }
+    destruct (decide (a < e))%a as [Hae|Hae]; cycle 1.
+    {
+      iApply (wp_store_fail_reg with "[HPC Hi Hdst Hsrc]")
+      ; try iFrame
+      ; try solve_pure.
+      { rewrite /withinBounds; solve_addr. }
+      iNext; iIntros "_".
+      iApply "Hφ"; by iLeft.
+    }
+
+    iDestruct (writeAllowed_valid_cap with "Hinterp_dst") as "%Hdst_in_region"; auto.
+    assert ( ∃ ρ, std W !! a = Some ρ ∧ ρ ≠ Revoked) as ( ρ & Hρ & Hρ_not_revoked).
+    {
+      rewrite Forall_lookup in Hdst_in_region.
+      assert ( a ∈ finz.seq_between b e) as Ha.
+      { apply elem_of_finz_seq_between; solve_addr. }
+      rewrite elem_of_list_lookup in Ha.
+      destruct Ha as [ka Hka].
+      apply Hdst_in_region in Hka.
+      done.
+    }
+
+    iDestruct (interp_has_rel _ _ _ _ _ _ _ a with "Hinterp_dst")
+      as (p_a φ_a)
+           "#(Hrel_a & Hφ_a_wcond & %Hpers_φ_a & %Hflow_p_a)".
+    { solve_addr. }
+    { done. }
+    iDestruct (region_open _ _ _ _ _ ρ with "[$Hrel_a $Hworld $Hregion]")
+      as (wastk) "(Hregion & Hworld & Hsts_std_a & Ha & _ & #Hmono_φ_a & Hφ_a)"; eauto.
+    { destruct ρ; naive_solver. }
+
+    iApply (wp_store_success_reg _ _ _ _ _ _ _ _ rdst rsrc with "[$HPC Hi Hsrc Hdst Ha]")
+    ; try iFrame
+    ; try solve_pure.
+    { rewrite /withinBounds; solve_addr. }
+    iNext; iIntros "(HPC & Hi & Hsrc & Hdst & Ha)".
+    iDestruct (region_close
+                with "[$Hsts_std_a $Hregion $Ha Hmono_φ_a $Hrel_a]")
+      as "Hregion".
+    { intros.
+      rewrite /persistent_cond in Hpers_φ_a.
+      specialize (Hpers_φ_a Wv); apply _.
+    }
+    { destruct ρ; naive_solver. }
+    { iSplit.
+      + iPureIntro; by eapply writeAllowed_nonO, writeAllowed_flowsto.
+      + admit. (* TODO see how it's done in the FTLR *)
+    }
+
+    iApply "Hφ"; iRight; iFrame "∗%".
+    iSplit; first done.
+    iPureIntro; solve_addr.
+  Admitted.
+
+  Lemma wp_unseal_unknown E pc_p pc_g pc_b pc_e pc_a pc_a' wi r1 r2 wsealr wsealed  :
+    decodeInstrW wi = UnSeal r2 r1 r2 →
+    isCorrectPC (WCap pc_p pc_g pc_b pc_e pc_a) →
+    (pc_a + 1)%a = Some pc_a' →
+
+    {{{  PC ↦ᵣ WCap pc_p pc_g pc_b pc_e pc_a
+          ∗ pc_a ↦ₐ wi
+          ∗ r1 ↦ᵣ wsealr
+          ∗ r2 ↦ᵣ wsealed
+    }}}
+      Instr Executable @ E
+      {{{ retv, RET retv;
+          ⌜ retv = FailedV ⌝
+          ∨ ∃ psr gsr bsr esr asr wsb,
+              ⌜ retv = NextIV ⌝
+              ∗ PC ↦ᵣ WCap pc_p pc_g pc_b pc_e pc_a'
+              ∗ r1 ↦ᵣ wsealr
+              ∗ r2 ↦ᵣ WSealable wsb
+              ∗ ⌜ wsealr = (WSealRange psr gsr bsr esr asr) ⌝ ∗ ⌜ permit_unseal psr = true ⌝
+              ∗ ⌜ wsealed = WSealed asr wsb ⌝
+      }}}.
+  Proof.
+    iIntros (Hinstr Hvpc Hpc_a' ϕ) "(HPC & Hpc_a & Hr1 & Hr2) Hφ".
+
+    iDestruct (map_of_regs_3 with "HPC Hr1 Hr2") as "[Hmap (%&%&%)]".
+    iApply (wp_UnSeal with "[$Hmap Hpc_a]"); eauto; simplify_map_eq; eauto.
+    by unfold regs_of; rewrite !dom_insert; set_solver+.
+    iNext. iIntros (regs' retv) "(#Hspec & Hpc_a & Hmap)". iDestruct "Hspec" as %Hspec.
+
+    destruct Hspec as [ | ]; iApply "Hφ"; [iRight | by iLeft].
+    rewrite lookup_insert_ne // lookup_insert  in H2.
+    rewrite lookup_insert_ne // lookup_insert_ne // lookup_insert in H3.
+    apply incrementPC_Some_inv in H6.
+    destruct H6 as ( ppc & gpc & bpc & epc & apc & apc' & HPC & Hapc' & ->).
+    rewrite lookup_insert_ne // lookup_insert in HPC.
+    simplify_eq.
+    iExists p, g, b, e, a, sb.
+    rewrite (insert_commute _ _ PC) //.
+    rewrite (insert_commute _ _ r1) //.
+    rewrite !insert_insert.
+    iDestruct (big_sepM_insert with "Hmap") as "[HPC Hmap]"; first by simplify_map_eq.
+    iDestruct (big_sepM_insert with "Hmap") as "[Hr1 Hmap]"; first by simplify_map_eq.
+    iDestruct (big_sepM_insert with "Hmap") as "[Hr2 Hmap]"; first by simplify_map_eq.
+    iFrame; done.
+  Qed.
+
+  Lemma wp_unseal_unknown_sealed E pc_p pc_g pc_b pc_e pc_a pc_a' wi r1 r2 psr gsr bsr esr asr wsealed  :
+    decodeInstrW wi = UnSeal r2 r1 r2 →
+    isCorrectPC (WCap pc_p pc_g pc_b pc_e pc_a) →
+    (pc_a + 1)%a = Some pc_a' →
+    permit_unseal psr = true ->
+    (bsr <= asr < esr)%ot ->
+
+    {{{  PC ↦ᵣ WCap pc_p pc_g pc_b pc_e pc_a
+          ∗ pc_a ↦ₐ wi
+          ∗ r1 ↦ᵣ WSealRange psr gsr bsr esr asr
+          ∗ r2 ↦ᵣ wsealed
+    }}}
+      Instr Executable @ E
+      {{{ retv, RET retv;
+          ⌜ retv = FailedV ⌝
+          ∨ ∃ wsb,
+              ⌜ retv = NextIV ⌝
+              ∗ PC ↦ᵣ WCap pc_p pc_g pc_b pc_e pc_a'
+              ∗ pc_a ↦ₐ wi
+              ∗ r1 ↦ᵣ WSealRange psr gsr bsr esr asr
+              ∗ r2 ↦ᵣ WSealable wsb
+              ∗ ⌜ wsealed = WSealed asr wsb ⌝
+      }}}.
+  Proof.
+    iIntros (Hinstr Hvpc Hpc_a' Hpsr Hsr ϕ) "(HPC & Hpc_a & Hr1 & Hr2) Hφ".
+
+    iDestruct (map_of_regs_3 with "HPC Hr1 Hr2") as "[Hmap (%&%&%)]".
+    iApply (wp_UnSeal with "[$Hmap Hpc_a]"); eauto; simplify_map_eq; eauto.
+    by unfold regs_of; rewrite !dom_insert; set_solver+.
+    iNext. iIntros (regs' retv) "(#Hspec & Hpc_a & Hmap)". iDestruct "Hspec" as %Hspec.
+
+    destruct Hspec as [ | ]; iApply "Hφ"; [iRight | by iLeft].
+    rewrite lookup_insert_ne // lookup_insert  in H2.
+    rewrite lookup_insert_ne // lookup_insert_ne // lookup_insert in H3.
+    apply incrementPC_Some_inv in H6.
+    destruct H6 as ( ppc & gpc & bpc & epc & apc & apc' & HPC & Hapc' & ->).
+    rewrite lookup_insert_ne // lookup_insert in HPC.
+    simplify_eq.
+    iExists sb.
+    rewrite (insert_commute _ _ PC) //.
+    rewrite (insert_commute _ _ r1) //.
+    rewrite !insert_insert.
+    iDestruct (big_sepM_insert with "Hmap") as "[HPC Hmap]"; first by simplify_map_eq.
+    iDestruct (big_sepM_insert with "Hmap") as "[Hr1 Hmap]"; first by simplify_map_eq.
+    iDestruct (big_sepM_insert with "Hmap") as "[Hr2 Hmap]"; first by simplify_map_eq.
+    iFrame; done.
+  Qed.
+
+
+
+  Set Nested Proofs Allowed.
   Lemma switcher_interp_expr (W : WORLD) (C : CmptName) (N : namespace) (rmap : Reg)
     (b_switcher e_switcher a_switcher_cc b_tstk e_tstk : Addr) (ot_switcher : OType) :
     na_inv logrel_nais N (switcher_inv b_switcher e_switcher a_switcher_cc b_tstk e_tstk ot_switcher) -∗
@@ -85,10 +314,8 @@ Section Switcher.
     iDestruct (big_sepM_delete _ _ cs1 with "Hrmap") as "[Hcs1 Hrmap]"; first by simplify_map_eq.
     assert (exists wct2, rmap !! ct2 = Some wct2) as [wct2 Hwct2] by (by specialize (Hfull_rmap ct2)).
     iDestruct (big_sepM_delete _ _ ct2 with "Hrmap") as "[Hct2 Hrmap]"; first by simplify_map_eq.
-
-    Set Nested Proofs Allowed.
-
-
+    assert (exists wctp, rmap !! ctp = Some wctp) as [wctp Hwctp] by (by specialize (Hfull_rmap ctp)).
+    iDestruct (big_sepM_delete _ _ ctp with "Hrmap") as "[Hctp Hrmap]"; first by simplify_map_eq.
 
     (* ------------------------------------------------ *)
     (* ----- Start the proof of the switcher here ----- *)
@@ -103,9 +330,10 @@ Section Switcher.
     { iApply "Hrmap_interp"; eauto; done. }
     iAssert (interp W C wcgp) as "#Hinterp_wcgp".
     { iApply "Hrmap_interp"; eauto; done. }
+    iAssert (interp W C wct1) as "#Hinterp_wct1".
+    { iApply "Hrmap_interp"; eauto; done. }
 
     focus_block_0 "Hcode" as "Hcode" "Hcont"; iHide "Hcont" as hcont.
-    (* ---- store csp cs0 ---- *)
     destruct (is_cap wcsp) eqn:His_cap_csp ; cycle 1.
     { (* if csp is not a stack, it fails *)
       iInstr_lookup "Hcode" as "Hi" "Hcode".
@@ -119,160 +347,693 @@ Section Switcher.
     destruct wcsp as [ | [ p_stk g_stk b_stk e_stk a_stk |] | |]; cbn in His_cap_csp; try congruence.
     clear His_cap_csp.
 
-    destruct (decide (b_stk <= a_stk))%a as [Hstk_ba|Hstk_ba]; cycle 1.
-    {
-      iInstr_lookup "Hcode" as "Hi" "Hcode".
-      wp_instr.
-      iApply (wp_store_fail_reg with "[HPC Hi Hcsp Hcs0]")
-      ; try iFrame
-      ; try solve_pure.
-      { rewrite /withinBounds; solve_addr. }
-      iNext; iIntros "_".
-      wp_pure; wp_end ; by iIntros (?).
-    }
-    destruct (decide (canStore p_stk wcs0 = true))%a as [Hstk_store_cs0|Hstk_store_cs0]; cycle 1.
-    {
-      iInstr_lookup "Hcode" as "Hi" "Hcode".
-      wp_instr.
-      iApply (wp_store_fail_reg_perm with "[HPC Hi Hcsp Hcs0]")
-      ; try iFrame
-      ; try solve_pure.
-      { by destruct ( canStore p_stk wcs0 ); auto. }
-      iNext; iIntros "_".
-      wp_pure; wp_end ; by iIntros (?).
-    }
-    pose proof ( canStore_writeAllowed p_stk wcs0 Hstk_store_cs0 ) as Hp_stk_wa.
-    destruct (decide ((a_stk) < e_stk))%a as [Hstk_a|Hstk_a]; cycle 1.
-    {
-      iInstr_lookup "Hcode" as "Hi" "Hcode".
-      wp_instr.
-      iApply (wp_store_fail_reg with "[HPC Hi Hcsp Hcs0]")
-      ; try iFrame
-      ; try solve_pure.
-      { rewrite /withinBounds; solve_addr. }
-      iNext; iIntros "_".
-      wp_pure; wp_end ; by iIntros (?).
-    }
-
-
-  iDestruct (writeAllowed_valid_cap with "Hinterp_wcsp") as "%Hstk_in_region"; auto.
-  assert ( ∃ ρ_a_stk, std W !! a_stk = Some ρ_a_stk ∧ ρ_a_stk ≠ Revoked) as ( ρ_a_stk & Hρ_a_stk & Hρ_a_stk_not_revoked).
-  {
-    rewrite Forall_lookup in Hstk_in_region.
-    assert ( a_stk ∈ finz.seq_between b_stk e_stk) as H_a_stk.
-    { apply elem_of_finz_seq_between; solve_addr. }
-    rewrite elem_of_list_lookup in H_a_stk.
-    destruct H_a_stk as [ka Hka].
-    apply Hstk_in_region in Hka.
-    done.
-  }
-
-  iDestruct (interp_has_rel _ _ _ _ _ _ _ a_stk with "Hinterp_wcsp")
-    as (p_a_stk φ_a_stk) "#(Hrel_a_stk & Hφ_a_stk_wcond & %Hpers_φ_a_stk & %Hflow_p_a_stk)".
-  { solve_addr. }
-  { done. }
-  iDestruct (region_open _ _ _ _ _ ρ_a_stk with "[$Hrel_a_stk $Hworld $Hregion]")
-    as (wastk) "(Hregion & Hworld & Hsts_std_a_stk & Ha_stk & _ & #Hmono_φ_a_stk & Hφ_a_stk)"; eauto.
-  { destruct ρ_a_stk; naive_solver. }
-
-  iInstr_lookup "Hcode" as "Hi" "Hcode".
-  wp_instr.
-  iApply (wp_store_success_reg _ _ _ _ _ _ _ _ csp cs0 with "[$HPC Hi Hcs0 Hcsp Ha_stk]")
-  ; try iFrame
-  ; try solve_pure.
-  { rewrite /withinBounds; solve_addr. }
-  iNext; iIntros "(HPC & Hi & Hcso0 & Hcsp & Ha_stk)".
-  iDestruct ("Hcode" with "Hi") as "Hcode".
-  wp_pure.
-  iDestruct (region_close
-              with "[$Hsts_std_a_stk $Hregion $Ha_stk Hmono_φ_a_stk $Hrel_a_stk]")
-    as "Hregion".
-  { intros.
-    rewrite /persistent_cond in Hpers_φ_a_stk.
-    specialize (Hpers_φ_a_stk Wv); apply _.
-  }
-  { destruct ρ_a_stk; naive_solver. }
-  { iSplit.
-    + iPureIntro; by eapply writeAllowed_nonO, writeAllowed_flowsto.
-    + admit. (* TODO see how it's done in the FTLR *)
-  }
-
-  (* ---- lea csp 1 ---- *)
-  iInstr "Hcode".
-  { transitivity (Some (a_stk ^+ 1%Z)%a); auto;solve_addr. }
-
-
-
-  (* ---- store csp cs1 ---- *)
-  destruct (decide (canStore p_stk wcs1 = true))%a as [Hstk_store_cs1|Hstk_store_cs1]; cycle 1.
-  {
+    (* ---- store csp cs0 ---- *)
     iInstr_lookup "Hcode" as "Hi" "Hcode".
     wp_instr.
-    iApply (wp_store_fail_reg_perm with "[HPC Hi Hcsp Hcs1]")
-    ; try iFrame
+    iApply (wp_store_interp with "[HPC Hi Hcsp Hcs0 $Hregion $Hworld Hinterp_wcsp $Hinterp_wcs0]")
+    ; try iFrame "∗#"
     ; try solve_pure.
-    { by destruct ( canStore p_stk wcs1 ); auto. }
-    iNext; iIntros "_".
-    wp_pure; wp_end ; by iIntros (?).
-  }
-  pose proof ( canStore_writeAllowed p_stk wcs1 Hstk_store_cs1 ) as Hp_stk_wa1.
-  destruct (decide ((a_stk ^+1)%a < e_stk))%a as [Hstk_a1|Hstk_a1]; cycle 1.
-  {
+    iNext
+    ; iIntros (retv) "[->|(-> & HPC & Hi & Hcs0 & Hcsp & Hregion & Hworld & %Hcanstore_cs0 & [%Hstk_ba0 %Hstk_a0e] )]"
+    ; wp_pure ; first (wp_end ; by iIntros (?)).
+    iDestruct ("Hcode" with "Hi") as "Hcode".
+
+    (* ---- lea csp 1 ---- *)
+    iInstr "Hcode".
+    { transitivity (Some (a_stk ^+ 1%Z)%a); auto;solve_addr. }
+
+    (* ---- store csp cs1 ---- *)
     iInstr_lookup "Hcode" as "Hi" "Hcode".
     wp_instr.
-    iApply (wp_store_fail_reg with "[HPC Hi Hcsp Hcs1]")
-    ; try iFrame
+    iApply (wp_store_interp with "[HPC Hi Hcsp Hcs1 $Hregion $Hworld Hinterp_wcsp $Hinterp_wcs1]")
+    ; try iFrame "∗#"
     ; try solve_pure.
-    { rewrite /withinBounds; solve_addr. }
-    iNext; iIntros "_".
-    wp_pure; wp_end ; by iIntros (?).
-  }
-  set (a_stk1 := (a_stk ^+ 1)%a).
-  assert ( ∃ ρ_a_stk1, std W !! a_stk1 = Some ρ_a_stk1 ∧ ρ_a_stk1 ≠ Revoked) as ( ρ_a_stk1 & Hρ_a_stk1 & Hρ_a_stk1_not_revoked).
-  {
-    rewrite Forall_lookup in Hstk_in_region.
-    assert ( a_stk1 ∈ finz.seq_between b_stk e_stk) as H_a_stk1.
-    { apply elem_of_finz_seq_between; subst a_stk1 ; solve_addr. }
-    rewrite elem_of_list_lookup in H_a_stk1.
-    destruct H_a_stk1 as [ka Hka].
-    apply Hstk_in_region in Hka.
-    done.
-  }
+    iNext
+    ; iIntros (retv) "[->|(-> & HPC & Hi & Hcs1 & Hcsp & Hregion & Hworld & %Hcanstore_cs1 & [_ %Hstk_a1e] )]"
+    ; wp_pure ; first (wp_end ; by iIntros (?)).
+    iDestruct ("Hcode" with "Hi") as "Hcode".
 
-  iDestruct (interp_has_rel _ _ _ _ _ _ _ (a_stk ^+ 1)%a with "Hinterp_wcsp")
-    as (p_a_stk1 φ_a_stk1)
-         "#(Hrel_a_stk1 & Hφ_a_stk_wcond0 & %Hpers_φ_a_stk1 & %Hflow_p_a_stk1)".
-  { solve_addr. }
-  { done. }
-  iDestruct (region_open _ _ _ _ _ ρ_a_stk1 with "[$Hrel_a_stk1 $Hworld $Hregion]")
-    as (wastk1) "(Hregion & Hworld & Hsts_std_a_stk1 & Ha_stk1 & _ & #Hmono_φ_a_stk1 & Hφ_a_stk1)"; eauto.
-  { destruct ρ_a_stk1; naive_solver. }
+    (* ---- lea csp 1 ---- *)
+    iInstr "Hcode".
+    { transitivity (Some (a_stk ^+ 2%Z)%a); auto;solve_addr. }
 
-  iInstr_lookup "Hcode" as "Hi" "Hcode".
-  wp_instr.
-  iApply (wp_store_success_reg _ _ _ _ _ _ _ _ csp cs1 with "[$HPC Hi Hcs1 Hcsp Ha_stk1]")
-  ; try iFrame
-  ; try solve_pure.
-  { rewrite /withinBounds; solve_addr. }
-  iNext; iIntros "(HPC & Hi & Hcs0 & Hcsp & Ha_stk1)".
-  iDestruct ("Hcode" with "Hi") as "Hcode".
-  wp_pure.
-  iDestruct (region_close
-              with "[$Hsts_std_a_stk1 $Hregion $Ha_stk1 Hmono_φ_a_stk1 $Hrel_a_stk1]")
-    as "Hregion".
-  { intros.
-    rewrite /persistent_cond in Hpers_φ_a_stk1.
-    specialize (Hpers_φ_a_stk1 Wv); apply _.
-  }
-  { destruct ρ_a_stk1; naive_solver. }
-  { iSplit.
-    + iPureIntro; by eapply writeAllowed_nonO, writeAllowed_flowsto.
-    + admit. (* TODO see how it's done in the FTLR *)
-  }
-  (* ---- lea csp 1 ---- *)
-  iInstr "Hcode".
-  { transitivity (Some (a_stk ^+ 2%Z)%a); auto;solve_addr. }
+    (* ---- store csp cra ---- *)
+    iInstr_lookup "Hcode" as "Hi" "Hcode".
+    wp_instr.
+    iApply (wp_store_interp with "[HPC Hi Hcsp Hcra $Hregion $Hworld Hinterp_wcsp $Hinterp_wcra]")
+    ; try iFrame "∗#"
+    ; try solve_pure.
+    iNext
+    ; iIntros (retv) "[->|(-> & HPC & Hi & Hcra & Hcsp & Hregion & Hworld & %Hcanstore_cra & [_ %Hstk_a2e] )]"
+    ; wp_pure ; first (wp_end ; by iIntros (?)).
+    iDestruct ("Hcode" with "Hi") as "Hcode".
 
+    (* ---- lea csp 1 ---- *)
+    iInstr "Hcode".
+    { transitivity (Some (a_stk ^+ 3%Z)%a); auto;solve_addr. }
+
+    (* ---- store csp cgp ---- *)
+    iInstr_lookup "Hcode" as "Hi" "Hcode".
+    wp_instr.
+    iApply (wp_store_interp with "[HPC Hi Hcsp Hcgp $Hregion $Hworld Hinterp_wcsp $Hinterp_wcgp]")
+    ; try iFrame "∗#"
+    ; try solve_pure.
+    iNext
+    ; iIntros (retv) "[->|(-> & HPC & Hi & Hcgp & Hcsp & Hregion & Hworld & %Hcanstore_cgp & [_ %Hstk_a3e] )]"
+    ; wp_pure ; first (wp_end ; by iIntros (?)).
+    iDestruct ("Hcode" with "Hi") as "Hcode".
+
+    (* ---- lea csp 1 ---- *)
+    iInstr "Hcode".
+    { transitivity (Some (a_stk ^+ 4%Z)%a); auto;solve_addr. }
+
+    (* --- getp ct2 csp --- *)
+    iInstr "Hcode".
+    (* --- mov ctp (encodePerm RWL) --- *)
+    iInstr "Hcode".
+    (* --- sub ct2 ct2 ctp --- *)
+    iInstr "Hcode".
+    destruct ( decide (p_stk = RWL)) as [-> |Hpstk]; cycle 1.
+    { (* pstk is not RWL - will fail *)
+      assert ( (encodePerm p_stk - encodePerm RWL)%Z ≠ 0%Z ) as Heq.
+      { intro Hcontra.
+        apply Hpstk.
+        assert ( encodePerm p_stk = encodePerm RWL )%Z by lia.
+        by apply encodePerm_inj in H1.
+      }
+      iInstr "Hcode".
+      { congruence. }
+      iInstr "Hcode".
+      wp_end ; by iIntros (?).
+    }
+    replace ((encodePerm RWL - encodePerm RWL)%Z) with 0%Z by lia.
+    (* --- jnz 2 ct2 --- *)
+    iInstr "Hcode".
+    (* --- jmp 2 --- *)
+    iInstr "Hcode".
+
+    (* --- getl ct2 csp --- *)
+    iInstr "Hcode".
+    (* --- mov ctp (encodeLoc Local) --- *)
+    iInstr "Hcode".
+    (* --- sub ct2 ct2 ctp --- *)
+    iInstr "Hcode".
+    destruct ( decide (g_stk = Local)) as [-> |Hgstk]; cycle 1.
+    { (* pstk is not RWL - will fail *)
+      assert ( (encodeLoc g_stk - encodeLoc Local)%Z ≠ 0%Z ) as Heq.
+      { intro Hcontra.
+        apply Hgstk.
+        assert ( encodeLoc g_stk = encodeLoc Local )%Z by lia.
+        by apply encodeLoc_inj in H1.
+      }
+      iInstr "Hcode".
+      { congruence. }
+      iInstr "Hcode".
+      wp_end ; by iIntros (?).
+    }
+    replace ((encodeLoc Local - encodeLoc Local)%Z) with 0%Z by lia.
+    (* --- jnz 2 ct2 --- *)
+    iInstr "Hcode".
+    (* --- jmp 2 --- *)
+    iInstr "Hcode".
+
+
+    (* --- readsr ct2 mtdc --- *)
+    iInstr "Hcode".
+
+    destruct (decide ((a_tstk ^+ 1) < e_tstk))%a as [Htstk_ae|Htstk_ae]; cycle 1.
+    { admit. (* NOTE will fail in the next upcoming instructions *) }
+    destruct (decide (b_tstk <= a_tstk))%a as [Htstk_ba|Htstk_ba]; cycle 1.
+    { admit. (* NOTE will fail in the next upcoming instructions *) }
+    iAssert (⌜ exists tstk_a1 tstk_next', (tstk_next = tstk_a1 :: tstk_next')⌝)%I
+      as %(tstk_a1 & tstk_next' & ->).
+    { iEval (rewrite /region_pointsto) in "Htstk".
+      iDestruct (big_sepL2_length with "Htstk") as %Hlen_tstk.
+      iPureIntro.
+      assert (0 < length (finz.seq_between (a_tstk ^+ 1)%a e_tstk)) as Hlen_tstk_ae.
+      { rewrite finz_seq_between_length.
+        (* assert (a_tstk^+1 < e_tstk)%a by solve_addr. *)
+        assert (a_tstk < e_tstk)%a by solve_addr.
+        (* rewrite finz_dist_S; last solve_addr. *)
+        rewrite finz_dist_S; last solve_addr; lia.
+      }
+      destruct tstk_next as [|stk_a1 tstk_next]; first (cbn in Hlen_tstk; lia).
+      exists stk_a1, tstk_next; done.
+    }
+    iDestruct (region_pointsto_cons with "Htstk") as "[Ha1_tstk Htstk]".
+    { transitivity (Some (a_tstk ^+ 2)%a); auto; solve_addr. }
+    { solve_addr. }
+
+    (* Lea ct2 1%Z; *)
+    iInstr "Hcode".
+    {  transitivity (Some (a_tstk ^+1)%a); solve_addr. }
+
+    (* Store ct2 csp; *)
+    iInstr "Hcode".
+    { rewrite /withinBounds andb_true_iff; solve_addr. }
+
+    (* WriteSR mtdc ct2; *)
+    iInstr "Hcode".
+
+    (* Zero out the callee's stack frame *)
+    (* GetE cs0 csp; *)
+    iInstr "Hcode".
+
+    (* GetA cs1 csp; *)
+    iInstr "Hcode".
+
+    (* Subseg csp cs1 cs0 *)
+    iInstr "Hcode" with "Hlc".
+    { rewrite /isWithin andb_true_iff; solve_addr. }
+
+    unfocus_block "Hcode" "Hcont" as "Hcode"; subst hcont.
+
+    focus_block 1 "Hcode" as a_clear_stk1 Ha_clear_stk1 "Hcode" "Hcont"; iHide "Hcont" as hcont.
+
+    iDestruct (writeLocalAllowed_valid_cap with "Hinterp_wcsp") as "%Hstk_in_region"; auto.
+    opose proof ( extract_temps_split_world W (finz.seq_between (a_stk ^+4)%a e_stk)) as
+      (ltemp_unknown & HNoDup_unk & W_temps).
+    { apply finz_seq_between_NoDup. }
+    { rewrite !Forall_lookup in Hstk_in_region |- *.
+      intros k a Hka.
+      apply elem_of_list_lookup_2 in Hka.
+      assert (a ∈ finz.seq_between b_stk e_stk) as Hka'.
+      { rewrite !elem_of_finz_seq_between in Hka |- *; solve_addr. }
+      apply elem_of_list_lookup_1 in Hka'.
+      destruct Hka' as [k' Hka'].
+      eapply Hstk_in_region; eauto.
+    }
+    set ( Wtemp := (ltemp_unknown ++ finz.seq_between (a_stk ^+ 4)%a e_stk) ).
+    (* 1) revoke the world *)
+
+    iMod ( monotone_revoke_keep _ C Wtemp with "[$Hworld $Hregion]") as "(Hworld & Hregion & Htemp)".
+    { by cbn. }
+    { iPureIntro.
+      intros k' a' Hk'; cbn.
+      apply W_temps.
+      apply elem_of_list_lookup.
+      by eexists.
+    }
+    rewrite revoke_resources_later
+    ; iMod (lc_fupd_elim_later with "Hlc Htemp") as "Htemp".
+    subst Wtemp.
+    iDestruct (big_sepL_app with "Htemp") as "[Htemp_unknown Htemp_stk]".
+    iDestruct (big_sepL_sep with "Htemp_stk") as "[Htemp_stk Hstk_revoked]".
+    iDestruct (region_addrs_exists with "Htemp_stk") as (lp) "Htemp_stk".
+    iDestruct (region_addrs_exists2 with "Htemp_stk") as (lφ) "[%Hlen_lφ Htemp_stk]".
+    iDestruct (big_sepL2_sep with "Htemp_stk") as "[Hpers_stk_φ Htemp_stk]".
+    iDestruct (big_sepL2_sep with "Htemp_stk") as "[Htemp_stk Hrel_stk]".
+    iDestruct (region_addrs_exists2 with "Htemp_stk") as (lw) "[%Hlen_lw Htemp_stk]".
+    iDestruct (big_sepL2_sep with "Htemp_stk") as "[Hlp_notO Htemp_stk]".
+    iDestruct (big_sepL2_sep with "Htemp_stk") as "[Hstk Hmono_stk]".
+    rewrite (big_sepL2_zip_snd_2 _ (zip lp lφ) lw (λ a w, a ↦ₐ w)%I); last by rewrite Hlen_lw.
+
+
+    iApply (clear_stack_spec with "[ - $HPC $Hcsp $Hcs0 $Hcs1 $Hcode $Hstk]"); eauto.
+    { solve_addr. }
+    { solve_addr. }
+    iNext ; iIntros "(HPC & Hcsp & Hcs0 & Hcs1 & Hcode & Hstk)".
+
+    iDestruct (sts_update_frm _ _ (W0.2 + 1) with "Hworld") as ">Hworld".
+    iMod (update_region_revoked_temp_pwl_multiple ⊤ _ _
+                 (finz.seq_between (a_stk ^+ 4)%a e_stk) (region_addrs_zeroes (a_stk ^+ 4)%a e_stk) RWL interpC
+                with "[$] [$] [Hstk Hstk_revoked Hpers_stk_φ Hrel_stk Hlp_notO Hmono_stk]") as "[Hregion Hworld]".
+    { done. }
+    { done. }
+    { apply finz_seq_between_NoDup. }
+    { admit. (* NOTE easy, but tedious *) }
+    iMod (monotone_close_list_region W _ _ ltemp_unknown
+                with "[] [$Hworld $Hregion Htemp_unknown]") as "[Hworld Hregion]".
+    { admit. (* should be OK *) }
+    { iDestruct (big_sepL_sep with "Htemp_unknown") as "[Htemp_unknown _]".
+      iFrame.
+    }
+    clear Hlen_lφ Hlen_lw.
+
+    iMod ( sts_alloc_loc _ C true frame_rel_pub frame_rel_pub frame_rel_priv with "Hworld")
+      as "(Hworld & %Hfresh_ι & %Hfresh_ι' & Hsts_loc_ι & #Hsts_rel_ι)".
+    rewrite -!/(frame_W (close_list ltemp_unknown (std_update_multiple (revoke W) (finz.seq_between (a_stk ^+ 4)%a e_stk) Temporary))).
+
+    set (W1 := (close_list ltemp_unknown (std_update_multiple (revoke W) (finz.seq_between (a_stk ^+ 4)%a e_stk) Temporary))).
+    set (W2 := frame_W W1).
+    set (ι := fresh_cus_name W1).
+
+    iDestruct (region_monotone _ _ W2 with "Hregion") as "Hregion".
+    { subst W2. rewrite /frame_W //=. }
+    { apply frame_W_related_sts_pub_world. }
+
+    unfocus_block "Hcode" "Hcont" as "Hcode"; subst hcont.
+
+
+    focus_block 2 "Hcode" as a_unseal Ha_unseal "Hcode" "Hcont"; iHide "Hcont" as hcont.
+    (* GetB cs1 PC *)
+    iInstr "Hcode".
+
+    (* GetA cs0 PC *)
+    iInstr "Hcode".
+
+    (* Sub cs1 cs1 cs0 *)
+    iInstr "Hcode".
+    (* Mov cs0 PC *)
+    iInstr "Hcode".
+    (* Lea cs0 cs1 *)
+    assert ( (a_unseal ^+ 3 + (b_switcher - (a_unseal ^+ 1)))%a = Some ( (b_switcher ^+ 2%Z)%a ))
+    as ?.
+    { solve_addr+H0 Ha_unseal H. }
+    iInstr "Hcode".
+
+    (* Lea cs0 (-2)%Z *)
+    iInstr "Hcode" with "Hlc".
+    { transitivity (Some b_switcher); solve_addr+H0 Ha_unseal H. }
+
+    (* Load cs0 cs0 *)
+    iInstr "Hcode" with "Hlc".
+    iEval (cbn) in "Hcs0".
+
+    (* UnSeal ct1 cs0 ct1 *)
+    (* subst Hwct1_caller. *)
+
+    iInstr_lookup "Hcode" as "Hi" "Hcode".
+    wp_instr.
+    iApply (wp_unseal_unknown_sealed with "[HPC Hi Hct1 Hcs0 ]")
+    ; try iFrame "∗"
+    ; try solve_pure.
+    { done. }
+    { solve_addr. }
+    iNext ; iIntros (retv) "[->|Hret]" ; first (wp_pure ; wp_end ; by iIntros (?)).
+    iDestruct "Hret" as (w_entry_point) "(-> & HPC & Hi & Hcs0 & Hct1 & ->)".
+    iDestruct ("Hcode" with "Hi") as "Hcode".
+    wp_pure.
+
+    (* iInstr "Hcode". *)
+    (* { done. (* TODO solve_pure *) } *)
+    (* { apply withinBounds_true_iff; solve_addr. (* TODO solve_pure *) } *)
+    (* rewrite Heq_entry_point. *)
+
+    iDestruct ( interp_monotone_sd W W2 with "[] [$Hinterp_wct1]" ) as "Hinterp_wct1'".
+    { iPureIntro. subst W2 W1.
+      admit. (* TODO should be fine *)  }
+    iEval (rewrite fixpoint_interp1_eq /= /interp_sb) in "Hinterp_wct1'".
+    iDestruct "Hinterp_wct1'"
+      as (Pct1 Hpers_Pct1) "(HmonoReq & Hseal_pred_Pct1 & HPct1')".
+    rewrite -bi.later_sep.
+    iDestruct "Hlc" as "[Hlc Hlc']".
+    assert (Persistent (Pct1 W2 C (WSealable w_entry_point))) as Hpers_Pct1'
+    by (by specialize (Hpers_Pct1 (W2,C,(WSealable w_entry_point)))).
+    assert (Persistent (Pct1 W2 C (borrow (WSealable w_entry_point)))) as Hpers_Pct1''
+    by (by specialize (Hpers_Pct1 (W2,C,(borrow (WSealable w_entry_point))))).
+    iMod (lc_fupd_elim_later with "Hlc' HPct1'") as "#[HPct1 HPct1_borrow]".
+    clear Hpers_Pct1' Hpers_Pct1''; iClear "HPct1'".
+    iDestruct (seal_pred_agree with "Hseal_pred_Pct1 Hp_ot_switcher") as "Hot_switcher_agree_later".
+    iSpecialize ("Hot_switcher_agree_later" $! (W2,C,WSealable w_entry_point)).
+    iMod (lc_fupd_elim_later with "Hlc Hot_switcher_agree_later") as "#Hot_switcher_agree".
+    iClear "Hot_switcher_agree_later".
+
+    rewrite /ot_switcher_prop.
+    iEval (rewrite /safeC /=) in "Hot_switcher_agree".
+    iRewrite "Hot_switcher_agree" in "HPct1".
+    rewrite /ot_switcher_propC /ot_switcher_prop.
+    iDestruct "HPct1" as (g_tbl b_tbl e_tbl a_tbl
+                         bpcc epcc bcgp ecgp nargs off_entry
+                            Heq_entry_point Hatbl Hbtbl Hbtbl1 Hnargs)
+                           "(#Hinv_pcc_B & #Hinv_cgp_B & #Hinv_entry_B_f & #Hjmp_callee_pc)".
+    iClear "Hot_switcher_agree".
+    cbn in Heq_entry_point.
+    rewrite !Heq_entry_point.
+
+
+    (* Load cs0 ct1 *)
+    wp_instr.
+    iInv "Hinv_entry_B_f" as ">Hatbl" "Hcls_atbl".
+    iInstr "Hcode".
+    { split ; first solve_pure.
+      rewrite /withinBounds; solve_addr. }
+    iEval (cbn) in "Hcs0".
+    iMod ("Hcls_atbl" with "Hatbl") as "_"; iModIntro.
+    wp_pure.
+
+    (* LAnd ct2 cs0 7%Z *)
+    iInstr "Hcode".
+
+    (* ShiftR cs0 cs0 3%Z *)
+    iInstr "Hcode".
+
+    replace ( (Z.land (encode_entry_point nargs off_entry) 7)) with nargs by admit.
+    replace ( (encode_entry_point nargs off_entry ≫ 3)%Z) with off_entry by admit.
+    (* TODO unclear why the above are true: should be properties of encode_entry_point *)
+    (* GetB cgp ct1 *)
+    iInstr "Hcode".
+
+    (* GetA cs1 ct1 *)
+    iInstr "Hcode".
+
+    (* Sub cs1 cgp cs1 *)
+    iInstr "Hcode".
+
+    (* Lea ct1 cs1 *)
+    iInstr "Hcode".
+    { transitivity (Some b_tbl); solve_addr+Hatbl. }
+
+    (* Load cra ct1 *)
+    wp_instr.
+    iInv "Hinv_pcc_B" as ">Hbtbl" "Hcls_btbl".
+    iInstr "Hcode".
+    { split ; first solve_pure.
+      rewrite /withinBounds; solve_addr+Hatbl. }
+    iEval (cbn) in "Hcra".
+    iMod ("Hcls_btbl" with "Hbtbl") as "_"; iModIntro.
+    wp_pure.
+
+    (* Lea ct1 1%Z *)
+    iInstr "Hcode".
+    { transitivity (Some (b_tbl ^+ 1)%a); solve_addr+Hbtbl1. }
+
+    (* Load cgp ct1 *)
+    wp_instr.
+    iInv "Hinv_cgp_B" as ">Hbtbl1" "Hcls_btbl1".
+    iInstr "Hcode".
+    { split ; first solve_pure.
+      rewrite /withinBounds; solve_addr+Hatbl Hbtbl1. }
+    iEval (cbn) in "Hcra".
+    iMod ("Hcls_btbl1" with "Hbtbl1") as "_"; iModIntro.
+    wp_pure.
+
+    (* Lea cra cs0 *)
+    iInstr "Hcode".
+    { transitivity (Some (bpcc ^+ off_entry)%a); last solve_addr. admit. }
+    (* TODO actually, it's fine if the offset fail, the machine fails...
+       we just need not to use iInstr, but instead manually choose the wp rule
+     *)
+
+    (* Add ct2 ct2 1%Z *)
+    iInstr "Hcode".
+
+    unfocus_block "Hcode" "Hcont" as "Hcode"; subst hcont.
+
+    focus_block 3 "Hcode" as a_clear_pre_reg1 Ha_clear_pre_reg1 "Hcode" "Hcont"; iHide "Hcont" as hcont.
+
+    assert (exists wca0, rmap !! ca0 = Some wca0) as [wca0 Hwca0] by (by specialize (Hfull_rmap ca0)).
+    iDestruct (big_sepM_delete _ _ ca0 with "Hrmap") as "[Hca0 Hrmap]"; first by simplify_map_eq.
+    assert (exists wca1, rmap !! ca1 = Some wca1) as [wca1 Hwca1] by (by specialize (Hfull_rmap ca1)).
+    iDestruct (big_sepM_delete _ _ ca1 with "Hrmap") as "[Hca1 Hrmap]"; first by simplify_map_eq.
+    assert (exists wca2, rmap !! ca2 = Some wca2) as [wca2 Hwca2] by (by specialize (Hfull_rmap ca2)).
+    iDestruct (big_sepM_delete _ _ ca2 with "Hrmap") as "[Hca2 Hrmap]"; first by simplify_map_eq.
+    assert (exists wca3, rmap !! ca3 = Some wca3) as [wca3 Hwca3] by (by specialize (Hfull_rmap ca3)).
+    iDestruct (big_sepM_delete _ _ ca3 with "Hrmap") as "[Hca3 Hrmap]"; first by simplify_map_eq.
+    assert (exists wca4, rmap !! ca4 = Some wca4) as [wca4 Hwca4] by (by specialize (Hfull_rmap ca4)).
+    iDestruct (big_sepM_delete _ _ ca4 with "Hrmap") as "[Hca4 Hrmap]"; first by simplify_map_eq.
+    assert (exists wca5, rmap !! ca5 = Some wca5) as [wca5 Hwca5] by (by specialize (Hfull_rmap ca5)).
+    iDestruct (big_sepM_delete _ _ ca5 with "Hrmap") as "[Hca5 Hrmap]"; first by simplify_map_eq.
+    assert (exists wct0, rmap !! ct0 = Some wct0) as [wct0 Hwct0] by (by specialize (Hfull_rmap ct0)).
+    iDestruct (big_sepM_delete _ _ ct0 with "Hrmap") as "[Hct0 Hrmap]"; first by simplify_map_eq.
+
+    iDestruct (map_of_regs_4 with "[$Hca0] [$Hca1] [$Hca2] [$Hca3] ") as "[Hargmap _]".
+    iDestruct (big_sepM_insert with "[$Hargmap $Hca4]") as "Hargmap"; first by simplify_map_eq.
+    iDestruct (big_sepM_insert with "[$Hargmap $Hca5]") as "Hargmap"; first by simplify_map_eq.
+    iDestruct (big_sepM_insert with "[$Hargmap $Hct0]") as "Hargmap"; first by simplify_map_eq.
+    set ( argmap := <[ct0:=wct0]> (<[ca5:=wca5]> (<[ca4:=wca4]> (<[ca0:=wca0]> (<[ca1:=wca1]> (<[ca2:=wca2]> (<[ca3:=wca3]> ∅)))))) ).
+    iAssert ( [∗ map] r↦w ∈ argmap, r ↦ᵣ w ∗ interp W2 C w)%I with "[Hargmap]" as "Hargmap".
+    { admit. (* NOTE easy enough *) }
+
+    iApply (clear_registers_pre_call_skip_spec with "[- $HPC $Hargmap $Hct2 $Hcode]"); try solve_pure.
+    { set_solver. }
+    { solve_addr. }
+    iNext; iIntros "H".
+    iDestruct "H" as (arg_rmap') "(%Harg_rmap' & HPC & Hct2 & Harg_rmap' & Hcode)".
+    unfocus_block "Hcode" "Hcont" as "Hcode"; subst hcont.
+
+    focus_block 4 "Hcode" as a_clear_pre_reg2 Ha_clear_pre_reg2 "Hcode" "Hcont"; iHide "Hcont" as hcont.
+
+    iDestruct (big_sepM_insert _ _ ctp with "[$Hrmap $Hctp]") as "Hrmap"; first by simplify_map_eq.
+    (* rewrite insert_delete_insert. *)
+    repeat (try (rewrite -delete_insert_ne ; last done)); rewrite insert_delete_insert.
+    iDestruct (big_sepM_insert _ _ ct2 with "[$Hrmap $Hct2]") as "Hrmap"; first by simplify_map_eq.
+    repeat (try (rewrite -delete_insert_ne ; last done)); rewrite insert_delete_insert.
+    iDestruct (big_sepM_insert _ _ ct1 with "[$Hrmap $Hct1]") as "Hrmap"; first by simplify_map_eq.
+    repeat (try (rewrite -delete_insert_ne ; last done)); rewrite insert_delete_insert.
+    iDestruct (big_sepM_insert _ _ cs0 with "[$Hrmap $Hcs0]") as "Hrmap"; first by simplify_map_eq.
+    repeat (try (rewrite -delete_insert_ne ; last done)); rewrite insert_delete_insert.
+    iDestruct (big_sepM_insert _ _ cs1 with "[$Hrmap $Hcs1]") as "Hrmap"; first by simplify_map_eq.
+    repeat (try (rewrite -delete_insert_ne ; last done)); rewrite insert_delete_insert.
+
+    iApply (clear_registers_pre_call_spec with "[- $HPC $Hrmap $Hcode]"); try solve_pure.
+    { clear -Harg_rmap' Hfull_rmap.
+      rewrite !dom_delete_L.
+      rewrite !dom_insert_L.
+      rewrite !dom_delete_L.
+      apply regmap_full_dom in Hfull_rmap.
+      rewrite Hfull_rmap.
+
+      rewrite -difference_difference_l_L.
+      do 4 rewrite union_assoc_L.
+      rewrite union_comm_L.
+      admit. (* TODO should be OK, but just need to do some gset manipulation *)
+      (* replace {[cs1; cs0; ct1; ct2; ctp]} *)
+      (*   with ({[cs1; cs0; ct1]} ∪ {[ct2; ctp]} : gset _) by set_solver. *)
+      (* replace ( (all_registers_s ∖ dom arg_rmap ∖ {[PC; cgp; cra; csp; cs0; cs1; ct1]}) *)
+      (*            ∪ ({[cs1; cs0; ct1]} ∪ {[ct2; ctp]})) *)
+      (*   with ( (all_registers_s ∖ dom arg_rmap ∖ {[PC; cgp; cra; csp; cs0; cs1; ct1]} *)
+      (*             ∪ {[cs1; cs0; ct1]}) ∪ {[ct2; ctp]}) by set_solver. *)
+      (* rewrite union_comm_L. *)
+      (* replace ( *)
+      (*    (all_registers_s ∖ dom arg_rmap ∖ {[PC; cgp; cra; csp; cs0; cs1; ct1]} ∪ {[cs1; cs0; ct1]}) *)
+      (*   ) *)
+      (*   with ( *)
+      (*    all_registers_s ∖ dom arg_rmap ∖ {[PC; cgp; cra; csp]} *)
+      (*   ). *)
+      (* 2:{ *)
+      (*   replace {[PC; cgp; cra; csp; cs0; cs1; ct1]} *)
+      (*   with ( {[PC; cgp; cra; csp]} ∪ {[cs1; cs0; ct1]} : gset _) *)
+      (*        by set_solver. *)
+      (* rewrite -(difference_difference_l_L  _ _ {[cs1; cs0; ct1]}). *)
+      (* rewrite difference_union_L. *)
+      (* set_solver. *)
+      (* } *)
+      (* rewrite subseteq_union_1_L; set_solver. *)
+    }
+    iNext; iIntros "H".
+    iDestruct "H" as (rmap') "(%Hrmap' & HPC & Hrmap' & Hcode)".
+    unfocus_block "Hcode" "Hcont" as "Hcode"; subst hcont.
+
+    focus_block 5 "Hcode" as a_jmp Ha_jmp "Hcode" "Hcont"; iHide "Hcont" as hcont.
+    set (
+        rmap'' :=
+       <[PC:=WCap RX Global bpcc epcc (bpcc ^+ off_entry)%a]>
+      (<[csp:=WCap RWL Local (a_stk ^+ 4)%a e_stk (a_stk ^+ 4)%a]>
+         (<[cra:=WSentry XSRW_ Local b_switcher e_switcher (a_jmp ^+ 1)%a]>
+            (<[cgp:=WCap RW Global bcgp ecgp bcgp]> (arg_rmap' ∪ rmap'))))
+      ).
+    iSpecialize ("Hjmp_callee_pc" $! W2 rmap'' (related_sts_priv_refl_world W2)).
+
+    (* Jalr cra cra *)
+    iInstr "Hcode".
+    unfocus_block "Hcode" "Hcont" as "Hcode"; subst hcont.
+    iEval (cbn) in "Hcgp".
+
+    iDestruct (tframe_agree with "Htframe_full Htframe_frag") as "->".
+    iDestruct (tframe_update _ _ (frm W + 1) with "Htframe_full Htframe_frag")
+                as ">[Htframe_full Htframe_frag]".
+    iMod ("Hclose_switcher_inv" with
+           "[$Hna Hmtdc Hcode Hb_switcher Htstk Htframe_full]")
+      as "Hna"
+    .
+    { iNext; iFrame "Hmtdc".
+      iExists (frm W + 1),tstk_next'.
+      iSplit; first done.
+      iSplit; first done.
+      iFrame.
+      replace ((a_tstk ^+ 1) ^+ 1)%a with (a_tstk ^+ 2)%a by solve_addr+Htstk_ae.
+      iFrame "∗#".
+      iPureIntro.
+      clear -H_tstk_frame Htstk_ba Htstk_ae Hbounds_tstk_b Hbounds_tstk_e.
+      split; replace a_tstk with (b_tstk ^+ frm W)%a; solve_addr.
+    }
+
+    set (Pframe := ((a_tstk ^+ 1)%a ↦ₐ WCap RWL Local b_stk e_stk (a_stk ^+ 4)%a)%I).
+    assert ( Nframe : namespace ). admit.
+    iMod (na_inv_alloc
+            logrel_nais
+            ⊤ (Nframe .@ ι)
+            (frame_inv C ι Pframe)
+           with "[$Hsts_loc_ι $Ha1_tstk ]") as "#Hinv_frame".
+
+    (* show that csp in safe-to-share *)
+    iAssert ( interp W2 C (WCap RWL Local (a_stk ^+ 4)%a e_stk (a_stk ^+ 4)%a)) as "Hinterp_csp".
+    { iApply (interp_monotone W).
+      + admit. (* TODO should be fine *)
+      + iApply (interp_weakeningEO with "Hinterp_wcsp"); auto.
+        * solve_addr+Hstk_a3e Hstk_ba0.
+        * solve_addr+Hstk_a3e Hstk_ba0.
+    }
+
+    iAssert (interp W2 C (WSentry XSRW_ Local b_switcher e_switcher (a_jmp ^+ 1)%a)) as "Hinterp_return".
+    { shelve. }
+
+    iDestruct (big_sepM_sep with "Harg_rmap'") as "[Harg_rmap' #Harg_rmap'_interp]".
+    iDestruct (big_sepM_sep with "Hrmap'") as "[Hrmap' %Hrmap'_zero]".
+    iCombine "Harg_rmap' Hrmap'" as "Hrmap'".
+
+    rewrite -(big_sepM_union _ arg_rmap' rmap').
+    2: {
+      clear -Harg_rmap' Hrmap'.
+      rewrite /is_arg_rmap in Harg_rmap'; simplify_eq.
+      apply map_disjoint_dom.
+      set_solver.
+    }
+    iDestruct (big_sepM_insert _ _ cgp with "[$Hrmap' $Hcgp]") as "Hrmap'".
+    {
+      clear -Harg_rmap' Hrmap'.
+      rewrite /is_arg_rmap in Harg_rmap'; simplify_eq.
+      rewrite /dom_arg_rmap in Hrmap'.
+      apply not_elem_of_dom.
+      set_solver.
+    }
+    iDestruct (big_sepM_insert _ _ cra with "[$Hrmap' $Hcra]") as "Hrmap'".
+    {
+      clear -Harg_rmap' Hrmap'.
+      rewrite /is_arg_rmap in Harg_rmap'; simplify_eq.
+      rewrite /dom_arg_rmap in Hrmap'.
+      apply not_elem_of_dom.
+      set_solver.
+    }
+    iDestruct (big_sepM_insert _ _ csp with "[$Hrmap' $Hcsp]") as "Hrmap'".
+    {
+      clear -Harg_rmap' Hrmap'.
+      rewrite /is_arg_rmap in Harg_rmap'; simplify_eq.
+      rewrite /dom_arg_rmap in Hrmap'.
+      do 2 rewrite lookup_insert_ne //.
+      apply not_elem_of_dom.
+      set_solver.
+    }
+    iDestruct (big_sepM_insert _ _ PC with "[$Hrmap' $HPC]") as "Hrmap'".
+    {
+      clear -Harg_rmap' Hrmap'.
+      rewrite /is_arg_rmap in Harg_rmap'; simplify_eq.
+      rewrite /dom_arg_rmap in Hrmap'.
+      do 3 rewrite lookup_insert_ne //.
+      apply not_elem_of_dom.
+      set_solver.
+    }
+
+    match goal with
+    | _ : _ |- context [<[PC:=?w]> ?m] =>
+        subst rmap'' ; set (rmap'' := <[PC:=w]> m)
+    end.
+
+
+    iApply "Hjmp_callee_pc"; iFrame.
+    iSplitR "Htframe_frag"; cycle 1.
+    { subst W2 W1. rewrite frame_W_lookup_frm /= std_update_multiple_frm /=. }
+    Lemma
+  tframe_frag (close_list ltemp_unknown (std_update_multiple (revoke W) (finz.seq_between (a_stk ^+ 4)%a e_stk) Temporary)).2
+
+    { rewrite /execute_entry_point_register; cbn.
+      iSplitR.
+      {
+        clear -Hrmap' Harg_rmap'.
+        subst hinv_switcher hφ0 htemp_unknown Pframe.
+        iPureIntro.
+        intros r; cbn.
+        destruct (decide (r = PC)) as [Hrpc | Hrpc]; simplify_eq; first by rewrite lookup_insert.
+        rewrite lookup_insert_ne //.
+        destruct (decide (r = csp)) as [Hrcsp | Hrcsp]; simplify_eq; first by rewrite lookup_insert.
+        rewrite lookup_insert_ne //.
+        destruct (decide (r = cra)) as [Hrcra | Hrcra]; simplify_eq; first by rewrite lookup_insert.
+        rewrite lookup_insert_ne //.
+        destruct (decide (r = cgp)) as [Hrcgp | Hrcgp]; simplify_eq; first by rewrite lookup_insert.
+        rewrite lookup_insert_ne //.
+        apply elem_of_dom.
+        rewrite dom_union.
+        rewrite elem_of_union.
+        destruct (decide (r ∈ dom arg_rmap')); first by left.
+        right.
+        rewrite Harg_rmap' in n.
+        assert (r ∉ ({[PC; cra; cgp; csp]} : gset RegName)).
+        { set_solver.  }
+        rewrite Hrmap'.
+        rewrite elem_of_difference.
+        split; first by apply all_registers_s_correct.
+        set_solver.
+      }
+      iSplitR.
+      { iPureIntro. by rewrite lookup_insert. }
+      iSplitR.
+      { iPureIntro.
+        subst rmap''.
+        do 3 (rewrite lookup_insert_ne //).
+        by rewrite lookup_insert.
+      }
+      iSplitR.
+      { iIntros (wstk Hcsp).
+        subst rmap''.
+        rewrite lookup_insert_ne // in Hcsp.
+        rewrite lookup_insert in Hcsp; simplify_eq.
+        iFrame "#".
+      }
+      iSplitR.
+      { iIntros (wret Hcra).
+        subst rmap''.
+        do 2 (rewrite lookup_insert_ne // in Hcra).
+        rewrite lookup_insert in Hcra; simplify_eq.
+        iFrame "#".
+      }
+
+      iSplitR.
+      { iIntros (r wr Hr_arg Hr).
+        subst rmap''.
+        iClear "Hjmp_callee_pc Hp_ot_switcher".
+        clear -Hr_arg Hr Harg_rmap' Hrmap'.
+        rewrite /dom_arg_rmap in Hr_arg.
+        destruct (decide (r = PC)) as [Hrpc|Hrpc]
+        ; first (exfalso ; set_solver+Hr_arg Hrpc).
+        destruct (decide (r = csp)) as [Hrcsp|Hrcsp]
+        ; first (exfalso ; set_solver+Hr_arg Hrcsp).
+        destruct (decide (r = cra)) as [Hrcra|Hrcra]
+        ; first (exfalso ; set_solver+Hr_arg Hrcra).
+        destruct (decide (r = cgp)) as [Hrcgp|Hrcgp]
+        ; first (exfalso ; set_solver+Hr_arg Hrcgp).
+        do 4 (rewrite lookup_insert_ne // in Hr).
+        rewrite lookup_union in Hr.
+        rewrite union_Some in Hr.
+        destruct Hr as [Hr | Hr]; cycle 1.
+        { exfalso.
+          destruct Hr as [Hcontra _].
+          rewrite /is_arg_rmap /dom_arg_rmap in Harg_rmap'.
+          rewrite -Harg_rmap' in Hr_arg.
+          apply lookup_lookup_total_dom in Hr_arg.
+          congruence.
+        }
+        rewrite big_sepM_lookup; eauto.
+      }
+      {
+        iIntros (r Hr); iPureIntro.
+        clear -Hr Harg_rmap' Hrmap' Hrmap'_zero.
+
+        rewrite not_elem_of_union in Hr.
+        destruct Hr as [Hr1 Hr2].
+        repeat (rewrite not_elem_of_union in Hr2).
+        repeat (rewrite not_elem_of_singleton in Hr2).
+        destruct Hr2 as [ [ [Hrpc Hrcra ] Hrcgp] Hrcsp] .
+        do 4 (rewrite lookup_insert_ne //).
+        rewrite lookup_union.
+        rewrite union_Some.
+        right.
+        split.
+        {
+        rewrite /is_arg_rmap in Harg_rmap'.
+        rewrite -Harg_rmap' not_elem_of_dom in Hr1.
+        done.
+        }
+        assert (is_Some (rmap' !! r)) as [wr Hr].
+        { rewrite -elem_of_dom.
+          rewrite Hrmap'.
+          rewrite elem_of_difference.
+          split ; first apply all_registers_s_correct.
+          set_solver.
+        }
+        eapply map_Forall_lookup_1 in Hrmap'_zero; eauto.
+        by simplify_eq.
+    }
 
   Qed.
 
